Iris/Iris/ProofMode/Classes.lean
@@ -241,10 +241,10 @@ For the IPM TC synthesis, it needs to be an `uncheckedInParam` since it should m
 if the user provides an mvar.
 -/
 @[ipm_class, rocq_alias FromModal]
-class FromModal {PROP1 : outParam <| uncheckedInParam <| Type _}
+class FromModal (io : InOut) {PROP1 : semiOutParamIPM io (Type _)}
     {PROP2} {α : outParam <| uncheckedInParam <| Type _}
-    [outParam <| uncheckedInParam <| BI PROP1] [BI PROP2] (φ : outParam Prop)
-    (M : outParam <| uncheckedInParam <| Modality PROP1 PROP2)
+    [uncheckedInParam <| BI PROP1] [BI PROP2] (φ : outParam Prop)
+    (M : semiOutParamIPM io (Modality PROP1 PROP2))
     (sel : outParam <| uncheckedInParam α) (P : PROP2) (Q : outParam PROP1) where
   from_modal : φ → M.M Q ⊢ P
 export FromModal (from_modal)
